#+LATEX_CLASS: general
#+TITLE: Лекция 1
#+AUTHOR: Ilya Yaroshevskiy

* Производящие функции
Последовательность \(a_0, a_1, a_2, \dots\). Запишем в виде ряда
\[ A(t) = a_0 + a_1 t + a_2 t^2 + \dots \], где \(A(t)\) --- *производящая функция*
#+begin_property org
\-
- \(A(t) = a_0 + a_1 t + a_2 t + \dots \)
- \(B(t) = b_0 + b_1 t + b_2 t + \dots \)
\[A(t) + B(t) = C(t)\]
\[ c_n = a_n + b_n \]
\[ C(t) = c_0 + c_1 t + c_2 t^2 + \dots \]
#+end_property
#+begin_property org
\-
- \(A(t) = a_0 + a_1 t + a_2 t + \dots \)
- \(B(t) = b_0 + b_1 t + b_2 t + \dots \)
\[ A(t) \cdot B(t) = C(t) \]
\[ (a_0 + a_1 t + a_2 t^2 + \dots)\cdot(b_0 + b_1 t + b_2 t^2) = \]
\[ = a_0b_0 + (a_0 b_1 + a_1 b_0) t + (a_0 b_2 + a_1 b_1 + a_2 b_0) t^2 + \dots \]
\[ c_n = \sum_{k = 0}^n a_kb_{n - k} \]
\[ C(t) = c_0 + c_1 t + c_2 t^2 + \dots \]
#+end_property
#+begin_property org
\-
- \(A(t) = a_0 + a_1 t + a_2 t + \dots \)
- \(B(t) = b_0 + b_1 t + b_2 t + \dots \), \(b_0 \neq 0\)
\[ \frac{A(t)}{B(t)} = C(t) \]
\[ C(t)\cdot B(t) = A(t) \]
\[ c_n = a_n - \sum_{k = 0}^{n - 1}c_k b_{n - k} \]
Если \(b_0 = 1\) и \(a_i, b_i \in \mathbb{Z}\), то \(c_i \in \mathbb{Z}\)
#+end_property
#+begin_property org
\-
- \(A(t) = a_0 + a_1 t + a_2 t + \dots \)
\[ A'(t) = a_1 + 2\cdot a_2 t + 3 \cdot a_3 t^2 + \dots \]
\[ a'_n = n\cdot a_n t^{n - 1} \]
#+end_property
#+begin_property org
\-
- \(A(t) = a_0 + a_1 t + a_2 t + \dots \)
\[ \int A(t) = a_0 t + \frac{1}{2} a_1 t^2 + \frac{1}{3} a_2 t^3 + \dots \]
\[ a'_n = \frac{1}{n + 1} \cdot a_n t^{n + 1} \]
#+end_property
#+begin_property org
\-
- \(A(t) = a_0 + a_1 t + a_2 t + \dots \)
- \(B(t) = b_0 + b_1 t + b_2 t + \dots \), \(b_0 = 0\)
\[ C(t) = A(B(t)) \]
\[ c_n = \sum_{k = 1}^n a_i \sum_{n=k_1 + k_2 + \dots + k_i} \prod_{j = 1}^i b_{k_j} \]

#+end_property


