#+LATEX_CLASS: general
#+TITLE: 20
#+AUTHOR: Ilya Yaroshevskiy

* 20
:PROPERTIES:
:UNNUMBERED:
:END:

\[ f_{n + 2} = f_{n + 1} + f_n \]
\[ f_{n + 1} = f_{n} + f_{n - 1} \Rightarrow f_{n - 1} = f_{n + 1} - f_n \]
\[ f_{n + 2}^2 + f_{n - 1}^2 = f_{n+1}^2 + 2f_{n + 1}f_n + f_n^2 + f_{n +1}^2 - 2f_{n + 1}f_n + f_n^2 = 2f_{n + 1}^2 + 2f_n^2 \]
\[ f_{n+2}^2 = 2f_{n + 1}^2 + 2f_n^2 - f_{n - 1}^2 \]
\[ f_{n}^2 = 2f_{n - 1}^2 + 2f_{n - 2}^2 - f_{n - 3}^2 \]
\[ g_n := f_n^2 \]
\[ g_n = 2g_{n - 1} + 2g_{n - 2} - g_{n - 3}\]
** Находим производящую функцию:
- $c_1 = 2$
- $c_2 = 2$
- $c_3 = -1$


- $g_0 = f_0^2 = 1$
- $g_1 = f_1^2 = 1$
- $g_2 = f_2^2 = 4$


- $p_0 = g_0 = 1$
- $p_1 = g_1 - g_0c_1 = 1 - 2\cdot 1 = -1$
- $p_2 = g_2 - (g_1c_1 + g_0c_2) = 4 - (2 + 2) = 0$

** Итого
\[ A(t) = \frac{1 - t}{1 - 2t - 2t^2 + t^3} \]

